Clean up, and one new lemma. (Can you spot it? :)

Isabelle/Grammar_defs.thy
@@ -4,6 +4,11 @@ theory Grammar_defs imports AList_ext
   "~~/src/HOL/Library/Product_ord"
 begin
 
+
+(*****************************************************************************
+  Types
+ *****************************************************************************)
+
 type_synonym ('t, 'v) production_rule = "('t \<times> 'v list)"
 type_synonym ('t, 'v) production_rules = "('t, 'v) production_rule list"
 type_synonym ('t, 'v) grammar = "('v \<times> ('t, 'v) production_rules) list"
@@ -11,25 +16,57 @@ type_synonym ('t, 'v) grammar = "('v \<times> ('t, 'v) production_rules) list"
 type_synonym ('t, 'v) norm_list = "('v \<times> (nat \<times> ('t, 'v) production_rule)) list"
 
 
+(*****************************************************************************
+  Grammar
+ *****************************************************************************)
+
 definition gram_valid :: "('t::linorder, 'v::linorder) grammar \<Rightarrow> bool" where
   "gram_valid gr \<equiv> is_typical_alist gr \<and>
-     (\<forall>g \<in> set gr. case g of (v, pr) \<Rightarrow> is_typical_alist pr \<and>
-       (\<forall>vs \<in> set (map snd pr). \<forall>v' \<in> set vs. v' \<in> fst ` set gr) \<and>
-       (\<exists>vs \<in> set (map snd pr). \<forall>v' \<in> set vs. v' < v))"
+     (\<forall>(v, rules) \<in> set gr. is_typical_alist rules \<and>
+       (\<forall>vs \<in> snd ` set rules. \<forall>v' \<in> set vs. v' \<in> fst ` set gr) \<and>
+       (\<exists>vs \<in> snd ` set rules. \<forall>v' \<in> set vs. v' < v))"
 
-definition norm_of_variables :: "('t, 'v) norm_list \<Rightarrow> 'v list \<Rightarrow> nat" where
-  "norm_of_variables norms vars \<equiv> listsum (map fst (map (\<lambda>v. of_key norms v) vars))"
+(* definition gram_max_vars :: "('t, 'v) grammar \<Rightarrow> nat" where
+  "gram_max_vars gr = Max (set (map (\<lambda>(_, rules). Max (set (map (\<lambda>(_, vs). length vs) rules))) gr))" *)
 
-definition norm_list_of_rules ::
+
+(*****************************************************************************
+  Norm calculation
+ *****************************************************************************)
+
+definition norm_sum :: "('t, 'v) norm_list \<Rightarrow> 'v list \<Rightarrow> nat" where
+  "norm_sum norms vars \<equiv> listsum (map fst (map (\<lambda>v. of_key norms v) vars))"
+
+definition norms_of_rules ::
   "('t, 'v) norm_list \<Rightarrow> ('t, 'v) production_rules \<Rightarrow> (nat \<times> ('t, 'v) production_rule) list" where
-  "norm_list_of_rules norms rules \<equiv>
+  "norms_of_rules norms rules \<equiv>
      let valid_rules = filter (\<lambda>(t, vs). \<forall>v \<in> set vs. v \<in> fst ` set norms) rules in
-     map (\<lambda>r. (1 + norm_of_variables norms (snd r), r)) valid_rules"
+     map (\<lambda>r. (1 + norm_sum norms (snd r), r)) valid_rules"
 
-definition norm_of_production_rules ::
+definition min_norm_of_rules where
+  "min_norm_of_rules norms rules = Min (set (norms_of_rules norms rules))"
+
+definition norms_of_grammar ::
   "('t :: linorder, 'v :: linorder) grammar \<Rightarrow> ('t, 'v) norm_list" where
-  "norm_of_production_rules gr \<equiv> (fold (\<lambda>(v, rules). \<lambda>norms.
-     norms@[(v, Min (set (norm_list_of_rules norms rules)))]) gr [])"
+  "norms_of_grammar gr \<equiv> (fold (\<lambda>(v, rules). \<lambda>ns. ns@[(v, min_norm_of_rules ns rules)]) gr [])"
+
+definition norm_of_variables :: "('t :: linorder, 'v :: linorder) grammar \<Rightarrow> 'v list \<Rightarrow> nat" where
+  "norm_of_variables gr vars \<equiv> norm_sum (norms_of_grammar gr) vars"
+
+function minimal_word_of_variables :: "('t :: linorder, nat) grammar \<Rightarrow> nat list \<Rightarrow> 't list" where
+  "minimal_word_of_variables gr [] = []"
+| "minimal_word_of_variables gr (vh#vt) = (
+     if gram_valid gr \<and> set (vh#vt) \<subseteq> fst ` set gr then
+       let norms = norms_of_grammar gr in
+       let (t, vars) = snd (of_key norms vh) in
+       t#(minimal_word_of_variables gr (vars@vt))
+     else [])"
+by pat_completeness auto
+
+
+(*****************************************************************************
+  Norm definition
+ *****************************************************************************)
 
 fun eat_word :: "('t, 'v) grammar \<Rightarrow> 't list \<Rightarrow> 'v list \<Rightarrow> ('t list \<times> 'v list)" where
   "eat_word gr (th#tt) (vh#vt) = (
@@ -39,24 +76,6 @@ fun eat_word :: "('t, 'v) grammar \<Rightarrow> 't list \<Rightarrow> 'v list \<
 | "eat_word gr t v = (t, v)"
 
 lemmas eat_word_induct = eat_word.induct[case_names normal nil_word nil_vars]
-
-(* definition gram_max_vars :: "('t, 'v) grammar \<Rightarrow> nat" where
-  "gram_max_vars gr = Max (set (map (\<lambda>(_, rules). Max (set (map (\<lambda>(_, vs). length vs) rules))) gr))" *)
-
-(* TODO: is there a function which finds a nat for a given 'v :: linorder? *)
-(* we need to know how many elements are smaller than a given v of type 'v *)
-(* definition max_norm_of_variables :: "('t, nat) grammar \<Rightarrow> nat list \<Rightarrow> nat" where
-  "max_norm_of_variables gr vs = listsum (map (\<lambda>v. ((gram_max_vars gr) + 1) ^ v) vs)" *)
-
-function minimal_word_of_variables :: "('t :: linorder, nat) grammar \<Rightarrow> nat list \<Rightarrow> 't list" where
-  "minimal_word_of_variables gr [] = []"
-| "minimal_word_of_variables gr (vh#vt) = (
-     if gram_valid gr \<and> set (vh#vt) \<subseteq> fst ` set gr then
-       let norms = norm_of_production_rules gr in
-       let (t, vars) = snd (of_key norms vh) in
-       t#(minimal_word_of_variables gr (vars@vt))
-     else [])"
-by pat_completeness auto
 
 definition word_in_variables :: "('t, 'v) grammar \<Rightarrow> 't list \<Rightarrow> 'v list \<Rightarrow> bool" where
   "word_in_variables gr w v \<equiv> eat_word gr w v = ([], [])"
@@ -71,22 +90,16 @@ definition norm :: "('t, 'v) grammar \<Rightarrow> 'v list \<Rightarrow> nat" wh
   "norm gr v \<equiv> Min {length w | w. word_in_variables gr w v}"
 
 
+(*****************************************************************************
+  Norm reduction
+ *****************************************************************************)
+
 fun norm_reduce :: "('t :: linorder, 'v :: linorder) grammar \<Rightarrow> 'v list \<Rightarrow> nat \<Rightarrow> 'v list" where
   "norm_reduce gr v 0 = v"
 | "norm_reduce gr [] (Suc p) = []"
 | "norm_reduce gr (vh#vt) (Suc p) = (
-     let (n, (_, v)) = of_key (norm_of_production_rules gr) vh in
+     let (n, (_, v)) = of_key (norms_of_grammar gr) vh in
      if Suc p < n then (norm_reduce gr v p) @ vt
      else norm_reduce gr vt (Suc p - n))"
-
-
-definition test_gr :: "(char, nat) grammar" where
-  "test_gr =
-   [(0, [(CHR ''a'', [])]),
-    (1, [(CHR ''b'', [0])])]"
-
-value "gram_valid test_gr"
-value "norm_of_production_rules test_gr"
-value "word_in_variables test_gr ''a'' [0]"
 
 end
