Isabelle/Grammar.thy
@@ -3,9 +3,107 @@ theory Grammar imports
   "Helpers"
 begin
 
+
+(*****************************************************************************
+  norm_sum
+ *****************************************************************************)
+
+lemma ns_singleton: "norm_sum ns [v] = fst (of_key ns v)"
+by (simp add: norm_sum_def)
+
+
+(*****************************************************************************
+  norms_of_rules
+ *****************************************************************************)
+
+lemma "snd ` set (norms_of_rules norms rules) \<subseteq> set rules"
+by (unfold norms_of_rules_def) auto
+
+lemma nor_nonempty:
+  "\<exists>(t, vs) \<in> set rules. \<forall>v \<in> set vs. v \<in> fst ` set norms \<Longrightarrow> norms_of_rules norms rules \<noteq> []"
+by (simp add: norms_of_rules_def filter_empty_conv)
+
+lemma "\<exists>a b. (a, b) \<in> set rules \<and> (\<forall>v\<in>set b. v \<in> fst ` set norms) \<Longrightarrow>
+  snd (Min (set (norms_of_rules norms rules))) \<in> set rules"
+by (rule Min_predicate) (auto simp add: norms_of_rules_def)
+
+
+(*****************************************************************************
+  min_norm_of_rules
+ *****************************************************************************)
+
+lemma
+  assumes "\<exists>vs \<in> snd ` set rules. \<forall>v \<in> set vs. v \<in> fst ` set norms"
+    shows "min_norm_of_rules norms rules \<in> set (norms_of_rules norms rules)" using assms
+  apply (auto simp add: min_norm_of_rules_def norms_of_rules_def)
+  apply (rule Min.closed)
+by (auto simp add: filter_empty_conv min_def)
+
+
+(*****************************************************************************
+  norms_of_grammar
+ *****************************************************************************)
+
+lemma "length (norms_of_grammar gr) = length gr"
+by (auto simp add: norms_of_grammar_def fold_concat_empty_init)
+
+lemma nog_fst_is_gr_fst: "map fst (norms_of_grammar gr) = map fst gr"
+by (auto simp add: norms_of_grammar_def
+    key_fold_empty_init[of _ "\<lambda>(v, rules) norms. min_norm_of_rules norms rules"])
+
+(* Do we need this? *)
+(* lemma nog_fst_is_gr_fst:
+  assumes "(v, n, t, vs) \<in> set (norms_of_grammar gr)"
+    shows "v \<in> fst ` set gr"
+proof -
+  have "fst ` set gr = set (map fst (norms_of_grammar gr))" by (simp add: nog_fst_is_gr_fst)
+  then show ?thesis using assms by (auto simp add: key_in_fst)
+qed *)
+
+
+(*****************************************************************************
+  norm_of_variables
+ *****************************************************************************)
+
+lemma nov_distr: "norm_of_variables gr (x @ y) = norm_of_variables gr x + norm_of_variables gr y"
+by (simp add: norm_of_variables_def norm_sum_def)
+
+lemma nov_distr': "norm_of_variables gr (x # y) = norm_of_variables gr [x] + norm_of_variables gr y"
+by (rule nov_distr[of _ "[x]", simplified])
+
+lemma nov_nog:
+  assumes "gram_valid gr"
+      and "(t, vs) = snd (of_key (norms_of_grammar gr) v)"
+      and "(v, rules) \<in> set gr"
+    shows "norm_of_variables gr vs < norm_of_variables gr [v]"
+  unfolding norm_of_variables_def norm_sum_def
+  apply simp
+sorry
+
+
+(*****************************************************************************
+  minimal_word_of_variables
+ *****************************************************************************)
+
+termination minimal_word_of_variables
+  apply (relation "measure (\<lambda>(gr, vs). norm_of_variables gr vs)", auto)
+  apply (subst nov_distr')
+  apply (simp add: nov_distr nov_nog)
+done
+
+
+(*****************************************************************************
+  eat_word
+ *****************************************************************************)
+
 (* The output word of eat_word is a postfix of the input word. *)
 lemma eat_word_postfix: "\<exists>p. w = p @ fst (eat_word gr w v)"
 by (induct gr w v rule: eat_word.induct, auto simp add: prefix_helper Let_def split_if_eq1)
+
+
+(*****************************************************************************
+  word_in_variables
+ *****************************************************************************)
 
 (* Postfixfreeness *)
 lemma postfix_free:
@@ -45,121 +143,22 @@ by (case_tac w) (auto simp add: word_in_variables_def)
 lemma no_word_no_variables: "(word_in_variables gr [] v) = (v = [])"
 by (case_tac v) (auto simp add: word_in_variables_def)
 
-lemma no_variables_zero_norm: "norm gr [] = 0"
-by (simp add: norm_def no_variables_no_word Min_eqI)
-
-
 lemma wiv_split: "word_in_variables gr w v \<Longrightarrow> word_in_variables gr w' v' \<Longrightarrow>
   word_in_variables gr (w@w') (v@v')"
 by (induct gr w v rule: eat_word.induct, auto simp add: word_in_variables_def Let_def split_if_eq1)
 
 
+(*****************************************************************************
+  norm
+ *****************************************************************************)
+
+lemma no_variables_zero_norm: "norm gr [] = 0"
+by (simp add: norm_def no_variables_no_word Min_eqI)
+
 lemma "gram_valid gr \<Longrightarrow> set a \<union> set b \<subseteq> fst ` set gr \<Longrightarrow> norm gr (a@b) = norm gr a + norm gr b"
 oops
 
-
-
-lemma "length (norms_of_grammar gr) = length gr"
-by (auto simp add: norms_of_grammar_def fold_concat_empty_init)
-
-lemma norm_fst_is_gr_fst: "map fst (norms_of_grammar gr) = map fst gr"
-by (auto simp add: norms_of_grammar_def
-    key_fold_empty_init[of _ "\<lambda>(v, rules) norms. Min (set (norms_of_rules norms rules))"])
-
-lemma "snd ` set (norms_of_rules norms rules) \<subseteq> set rules"
-by (unfold norms_of_rules_def) auto
-
-lemma nor_nonempty:
-  "\<exists>(t, vs) \<in> set rules. \<forall>v \<in> set vs. v \<in> fst ` set norms \<Longrightarrow> norms_of_rules norms rules \<noteq> []"
-by (simp add: norms_of_rules_def filter_empty_conv)
-
-lemma nog_fst_is_gr_fst:
-  assumes "(v, n, t, vs) \<in> set (norms_of_grammar gr)"
-    shows "v \<in> fst ` set gr"
-proof -
-  have "fst ` set gr = set (map fst (norms_of_grammar gr))" by (simp add: norm_fst_is_gr_fst)
-  then show ?thesis using assms by (auto simp add: key_in_fst)
-qed
-
-
-
-lemma helper: "\<exists>a b. (a, b) \<in> set rules \<and> (\<forall>v\<in>set b. v \<in> fst ` set norms) \<Longrightarrow>
-  snd (Min (set (norms_of_rules norms rules))) \<in> set rules"
-by (rule Min_predicate) (auto simp add: norms_of_rules_def)
-
-
-(* lemma
-  assumes G: "gram_valid gr"
-      and N: "(v, n, t, vs) \<in> set (norms_of_grammar gr)"
-    shows "(t, vs) \<in> set (of_key gr v)"
-proof -
-  have XX: "\<forall>(k, v)\<in>set gr. is_alist v" using G by (auto simp add: gram_valid_def is_typical_alist_def)
-  have XY: "v \<in> fst ` set gr" using G N by (simp add: nog_fst_is_gr_fst)
-  have AL: "is_alist (of_key gr v)" using XX XY by (rule of_key_forall)
-
-  have T1: "\<And>x. gram_valid gr \<Longrightarrow> x \<in> set gr \<Longrightarrow> case x of (v, rules) \<Rightarrow> of_key gr v = rules"
-    by (auto simp add: of_key_from_existence gram_valid_def is_typical_alist_def)
-  have T2: "\<And>P. \<forall>x\<in>set []. P x" by auto
-
-  have ABC: "\<And>a norms. \<forall>(v, n, t, vs)\<in>set norms. t \<in> fst ` set (of_key gr v) \<Longrightarrow>
-             \<exists>(n, t, vs) \<in> (set (norms_of_rules norms (of_key gr a))). True" sorry
-
-  have XYZ: "\<And>a s ab ac ba. \<forall>(v, n, t, vs)\<in>set s. t \<in> fst ` set (of_key gr v) \<Longrightarrow>
-             (ab, ac, ba) = Min (set (norms_of_rules s (of_key gr a))) \<Longrightarrow>
-             ac \<in> fst ` set (of_key gr a)" using G ABC by (auto simp add: Min.closed nor_nonempty norms_of_rules_def) (* TODO! *)
-
-  have T3: "\<And>x s. gram_valid gr \<Longrightarrow>
-          case x of (v, rules) \<Rightarrow> of_key gr v = rules \<Longrightarrow>
-          \<forall>(v, n, t, vs)\<in>set s. t \<in> fst ` set (of_key gr v) \<Longrightarrow>
-          \<forall>(v, n, t, vs)\<in>set ((\<lambda>(v, rules) norms. norms @ [(v, Min (set (norms_of_rules norms rules)))]) x s).
-             t \<in> fst ` set (of_key gr v)" using G XYZ by auto
-
-  have SGX: "gram_valid gr \<Longrightarrow>
-    \<forall>(v, n, t, vs)\<in>set (norms_of_grammar gr).
-      t \<in> fst ` set (of_key gr v)" unfolding norms_of_grammar_def using T1 T2 T3
-    by (rule fold_invariant[of _ "\<lambda>(v, rules). of_key gr v = rules"
-      "\<lambda>s. \<forall>(v, n, t, vs) \<in> set s. t \<in> fst ` set (of_key gr v)" _])
-
-  have SG: "\<forall>(v, n, t, vs) \<in> set (norms_of_grammar gr). t \<in> fst ` set (of_key gr v)"
-    using G SGX by (auto simp add: norms_of_grammar_def)
-
-  have EX1: "t \<in> fst ` set (of_key gr v)" using N SG by auto
-  have EX2: "of_key (of_key gr v) t = vs" sorry
-  show ?thesis using AL EX1 EX2 by (rule existence_from_of_key)
-qed *)
-
-(* lemma ns_distr: "norm_sum ns (x @ y) = norm_sum ns x + norm_sum ns y"
-by (simp add: norm_sum_def)
-
-lemma ns_distr': "norm_sum ns (x # y) = norm_sum ns [x] + norm_sum ns y"
-by (rule ns_distr[of _ "[x]", simplified]) *)
-
-lemma ns_singleton: "norm_sum ns [v] = fst (of_key ns v)"
-by (simp add: norm_sum_def)
-
-lemma nov_distr: "norm_of_variables gr (x @ y) = norm_of_variables gr x + norm_of_variables gr y"
-by (simp add: norm_of_variables_def norm_sum_def)
-
-lemma nov_distr': "norm_of_variables gr (x # y) = norm_of_variables gr [x] + norm_of_variables gr y"
-by (rule nov_distr[of _ "[x]", simplified])
-
-lemma nog_nov:
-  assumes "gram_valid gr"
-      and "(t, vs) = snd (of_key (norms_of_grammar gr) v)"
-      and "(v, rules) \<in> set gr"
-    shows "norm_of_variables gr vs < norm_of_variables gr [v]"
-  unfolding norm_of_variables_def norm_sum_def
-  apply simp
-sorry
-
-termination minimal_word_of_variables
-  apply (relation "measure (\<lambda>(gr, vs). norm_of_variables gr vs)", auto)
-  apply (subst nov_distr')
-  apply (simp add: nov_distr nog_nov)
-done
-
-
-lemma nov_norm_equal:
+lemma nov_calculates_norm:
   assumes G: "gram_valid gr"
       and V: "set v \<subseteq> fst ` set gr"
     shows "norm_of_variables gr v = norm gr v"
