Isabelle/Tests.thy
@@ -1,0 +1,13 @@
+theory Tests imports Grammar
+begin
+
+definition test_gr :: "(char, nat) grammar" where
+  "test_gr =
+   [(0, [(CHR ''a'', [])]),
+    (1, [(CHR ''b'', [0])])]"
+
+value "gram_valid test_gr"
+value "norms_of_grammar test_gr"
+value "word_in_variables test_gr ''a'' [0]"
+
+end
